% !TEX program = pdflatex
\documentclass[aspectratio=169]{beamer}
\usetheme{Madrid}
\usecolortheme{default}
\usepackage{tikz}

% Custom colors
\definecolor{myblue}{RGB}{0,114,178}
\definecolor{myorange}{RGB}{230,159,0}
\definecolor{mygreen}{RGB}{0,158,115}
\definecolor{myred}{RGB}{213,94,0}
\definecolor{mypurple}{RGB}{204,121,167}
\definecolor{mybrown}{RGB}{240,228,66}
\definecolor{mygray}{RGB}{189,189,189}

% Set colors
\setbeamercolor{title}{fg=white,bg=myblue}
\setbeamercolor{frametitle}{fg=white,bg=myblue}
\setbeamercolor{section title}{fg=white,bg=myblue}
\setbeamercolor{subsection title}{fg=white,bg=myorange}
\setbeamercolor{item}{fg=myblue}
\setbeamercolor{subitem}{fg=myorange}

% Remove navigation symbols
\setbeamertemplate{navigation symbols}{}

% Custom commands
\newcommand{\limx}[2]{\lim_{x \to #1} #2}

% Title page
\title{Arithmetic of Derivatives}
\subtitle{A Differentiation Toolbox}
\author{Differential Calculus}
\date{}

\begin{document}

\begin{frame}
\titlepage
\end{frame}

\begin{frame}{Outline}
\tableofcontents
\end{frame}

\section{Introduction}

\begin{frame}{Why We Need Differentiation Rules}
\begin{itemize}
  \item Computing derivatives using the limit definition becomes unwieldy for complex functions
  \item We need efficient tools to break down complicated derivatives into simple ones
  \item Similar to how we used "arithmetic of limits" for computing limits
\end{itemize}
\end{frame}

\begin{frame}{Basic Derivatives We Know}
\begin{block}{Simple Functions}
\[
\begin{aligned}
  \frac{d}{dx} 1 &= 0 \\
  \frac{d}{dx} x &= 1 \\
  \frac{d}{dx} x^2 &= 2x \\
  \frac{d}{dx} \sqrt{x} &= \frac{1}{2\sqrt{x}}
\end{aligned}
\]
\end{block}
\end{frame}

\section{Linearity of Differentiation}

\begin{frame}{Derivative of Sum and Difference}
\begin{block}{Lemma 2.4.1}
Let $f(x)$, $g(x)$ be differentiable functions and let $c \in \mathbb{R}$ be a constant. Then:
\[
\begin{aligned}
  \frac{d}{dx}[f(x) + g(x)] &= f'(x) + g'(x) \\
  \frac{d}{dx}[f(x) - g(x)] &= f'(x) - g'(x) \\
  \frac{d}{dx}[c \cdot f(x)] &= c \cdot f'(x)
\end{aligned}
\]
\end{block}
\end{frame}

\begin{frame}{Linearity of Differentiation}
\begin{block}{Theorem 2.4.2}
Let $f(x)$, $g(x)$ be differentiable functions, let $\alpha, \beta \in \mathbb{R}$ be constants and define:
\[
S(x) = \alpha f(x) + \beta g(x)
\]
Then:
\[
\frac{dS}{dx} = S'(x) = \alpha f'(x) + \beta g'(x)
\]
\end{block}
\end{frame}

\section{Product Rule}

\begin{frame}{The Product Rule}
\begin{block}{Theorem 2.4.3}
Let $f(x)$, $g(x)$ be differentiable functions, then:
\[
\frac{d}{dx}[f(x) \cdot g(x)] = f'(x) \cdot g(x) + f(x) \cdot g'(x)
\]
\end{block}
\begin{itemize}
  \item The derivative of a product is NOT the product of derivatives
  \item Remember: "First times derivative of second, plus second times derivative of first"
\end{itemize}
\end{frame}

\begin{frame}{Special Case: Derivative of a Square}
\begin{block}{Corollary 2.4.4}
Let $f(x)$ be a differentiable function, then:
\[
\frac{d}{dx}[f(x)]^2 = 2f(x) \cdot f'(x)
\]
\end{block}
\end{frame}

\section{Quotient Rule}

\begin{frame}{The Quotient Rule}
\begin{block}{Theorem 2.4.5}
Let $f(x)$, $g(x)$ be differentiable functions, then:
\[
\frac{d}{dx}\left[\frac{f(x)}{g(x)}\right] = \frac{f'(x) \cdot g(x) - f(x) \cdot g'(x)}{[g(x)]^2}
\]
\end{block}
\begin{itemize}
  \item This derivative exists except at points where $g(x) = 0$
  \item Remember: "Low d-high minus high d-low, over low squared"
\end{itemize}
\end{frame}

\begin{frame}{Special Case: Derivative of a Reciprocal}
\begin{block}{Corollary 2.4.6}
Let $g(x)$ be a differentiable function, then:
\[
\frac{d}{dx}\left[\frac{1}{g(x)}\right] = -\frac{g'(x)}{[g(x)]^2}
\]
\end{block}
\end{frame}

\section{Examples}

\begin{frame}{Example 1: Using Linearity}
\textbf{Find the derivative of } $f(x) = 3x^2 + 5x - 2$
\end{frame}

\begin{frame}{Solution to Example 1}
\textbf{Solution:}
\[
\begin{aligned}
  f(x) &= 3x^2 + 5x - 2 \\
  f'(x) &= \frac{d}{dx}(3x^2) + \frac{d}{dx}(5x) + \frac{d}{dx}(-2) \\
  &= 3 \cdot \frac{d}{dx}(x^2) + 5 \cdot \frac{d}{dx}(x) + 0 \\
  &= 3 \cdot 2x + 5 \cdot 1 \\
  &= 6x + 5
\end{aligned}
\]
\end{frame}

\begin{frame}{Example 2: Using Product Rule}
\textbf{Find the derivative of } $f(x) = x^2 \cdot \sqrt{x}$
\end{frame}

\begin{frame}{Solution to Example 2}
\textbf{Solution:}
\[
\begin{aligned}
  f(x) &= x^2 \cdot \sqrt{x} \\
  f'(x) &= \frac{d}{dx}(x^2) \cdot \sqrt{x} + x^2 \cdot \frac{d}{dx}(\sqrt{x}) \\
  &= 2x \cdot \sqrt{x} + x^2 \cdot \frac{1}{2\sqrt{x}} \\
  &= 2x\sqrt{x} + \frac{x^2}{2\sqrt{x}} \\
  &= 2x\sqrt{x} + \frac{x\sqrt{x}}{2} \\
  &= \frac{5x\sqrt{x}}{2}
\end{aligned}
\]
\end{frame}

\begin{frame}{Example 3: Using Quotient Rule}
\textbf{Find the derivative of } $f(x) = \frac{x^2 + 1}{x - 1}$
\end{frame}

\begin{frame}{Solution to Example 3}
\textbf{Solution:}
\[
\begin{aligned}
  f(x) &= \frac{x^2 + 1}{x - 1} \\
  f'(x) &= \frac{\frac{d}{dx}(x^2 + 1) \cdot (x-1) - (x^2 + 1) \cdot \frac{d}{dx}(x-1)}{(x-1)^2} \\
  &= \frac{2x \cdot (x-1) - (x^2 + 1) \cdot 1}{(x-1)^2} \\
  &= \frac{2x^2 - 2x - x^2 - 1}{(x-1)^2} \\
  &= \frac{x^2 - 2x - 1}{(x-1)^2}
\end{aligned}
\]
\end{frame}

\section{Practice Problems}

\begin{frame}{Practice: 1 and 2}
\textbf{Practice 1:}
\[
\text{Find the derivative of } f(x) = 4x^3 - 2x^2 + 7x - 3
\]
\vspace{1em}
\textbf{Practice 2:}
\[
\text{Find the derivative of } f(x) = x^3 \cdot (x^2 + 1)
\]
\end{frame}

\begin{frame}{Practice: 3 and 4}
\textbf{Practice 3:}
\[
\text{Find the derivative of } f(x) = \frac{x^2 - 4}{x + 2}
\]
\vspace{1em}
\textbf{Practice 4:}
\[
\text{Find the derivative of } f(x) = \frac{1}{x^2 + 1}
\]
\end{frame}

\begin{frame}{Practice: 5}
\textbf{Practice 5:}
\[
\text{Find the derivative of } f(x) = (x^2 + 3x)(x^3 - 2)
\]
\end{frame}

\begin{frame}{Practice: 6 and 7}
\textbf{Practice 6:}
\[
\text{Find the derivative of } f(x) = \frac{x^3 + 2x}{x^2 - 1}
\]
\vspace{1em}
\textbf{Practice 7:}
\[
\text{Find the derivative of } f(x) = (x^2 + 1)^2
\]
\end{frame}

\begin{frame}{Practice: 8 and 9}
\textbf{Practice 8:}
\[
\text{Find the derivative of } f(x) = \frac{1}{x^3 + 3x}
\]
\vspace{1em}
\textbf{Practice 9:}
\[
\text{Find the derivative of } f(x) = x^2 \cdot \sqrt{x^2 + 1}
\]
\end{frame}

\begin{frame}{Practice: 10 and 11}
\textbf{Practice 10:}
\[
\text{Find the derivative of } f(x) = \frac{\sqrt{x}}{x^2 + 1}
\]
\vspace{1em}
\textbf{Practice 11:}
\[
\text{Find the derivative of } f(x) = (x^3 - 2x)(x^2 + 3)^2
\]
\end{frame}

\begin{frame}{Practice: 12 and 13}
\textbf{Practice 12:}
\[
\text{Find the derivative of } f(x) = \frac{x^2 - 4}{x^2 + 4}
\]
\vspace{1em}
\textbf{Practice 13:}
\[
\text{Find the derivative of } f(x) = \frac{1}{(x^2 + 1)^2}
\]
\end{frame}

\begin{frame}{Practice: 14 and 15}
\textbf{Practice 14:}
\[
\text{Find the derivative of } f(x) = x \cdot \sqrt{x^2 - 1}
\]
\vspace{1em}
\textbf{Practice 15:}
\[
\text{Find the derivative of } f(x) = \frac{x^3 + x}{x^2 - x + 1}
\]
\end{frame}

% 新增三角函数、指数、对数、反三角函数练习题
\begin{frame}{Practice: 16 and 17}
\textbf{Practice 16:}
\[
\text{Find the derivative of } f(x) = x^2 \sin(x)
\]
\vspace{1em}
\textbf{Practice 17:}
\[
\text{Find the derivative of } f(x) = e^x \cos(x)
\]
\end{frame}

\begin{frame}{Practice: 18 and 19}
\textbf{Practice 18:}
\[
\text{Find the derivative of } f(x) = \ln(x^2 + 1)
\]
\vspace{1em}
\textbf{Practice 19:}
\[
\text{Find the derivative of } f(x) = \frac{\sin(x)}{x}
\]
\end{frame}

\begin{frame}{Practice: 20 and 21}
\textbf{Practice 20:}
\[
\text{Find the derivative of } f(x) = \arctan(x^2)
\]
\vspace{1em}
\textbf{Practice 21:}
\[
\text{Find the derivative of } f(x) = x \cdot e^x
\]
\end{frame}

\begin{frame}{Practice: 22 and 23}
\textbf{Practice 22:}
\[
\text{Find the derivative of } f(x) = \frac{\ln(x)}{x}
\]
\vspace{1em}
\textbf{Practice 23:}
\[
\text{Find the derivative of } f(x) = \arcsin(\sqrt{x})
\]
\end{frame}

\begin{frame}{Practice: 24 and 25}
\textbf{Practice 24:}
\[
\text{Find the derivative of } f(x) = \sin(x) \cos(x)
\]
\vspace{1em}
\textbf{Practice 25:}
\[
\text{Find the derivative of } f(x) = \frac{e^x}{x^2 + 1}
\]
\end{frame}

\section{Solutions to Practice Problems}

\begin{frame}{Solution to Practice 1}
\textbf{Practice 1:}

Find the derivative of $f(x) = 4x^3 - 2x^2 + 7x - 3$

\textbf{Solution:}
\[
\begin{aligned}
  f'(x) &= \frac{d}{dx}(4x^3) - \frac{d}{dx}(2x^2) + \frac{d}{dx}(7x) - \frac{d}{dx}(3) \\
  &= 4 \cdot 3x^2 - 2 \cdot 2x + 7 \cdot 1 - 0 \\
  &= 12x^2 - 4x + 7
\end{aligned}
\]
\end{frame}

\begin{frame}{Solution to Practice 2 (Part 1)}
\textbf{Practice 2:}

Find the derivative of $f(x) = x^3 \cdot (x^2 + 1)$

\textbf{Solution:}
\[
\begin{aligned}
  f'(x) &= \frac{d}{dx}(x^3) \cdot (x^2 + 1) + x^3 \cdot \frac{d}{dx}(x^2 + 1) \\
  &= 3x^2 \cdot (x^2 + 1) + x^3 \cdot 2x
\end{aligned}
\]
\end{frame}

\begin{frame}{Solution to Practice 2 (Part 2)}
\textbf{Solution (continued):}
\[
\begin{aligned}
  &= 3x^4 + 3x^2 + 2x^4 \\
  &= 5x^4 + 3x^2
\end{aligned}
\]
\end{frame}

\begin{frame}{Solution to Practice 3 (Part 1)}
\textbf{Practice 3:}

Find the derivative of $f(x) = \frac{x^2 - 4}{x + 2}$

\textbf{Solution:}
\[
\begin{aligned}
  f'(x) &= \frac{\frac{d}{dx}(x^2 - 4) \cdot (x+2) - (x^2 - 4) \cdot \frac{d}{dx}(x+2)}{(x+2)^2} \\
  &= \frac{2x \cdot (x+2) - (x^2 - 4) \cdot 1}{(x+2)^2}
\end{aligned}
\]
\end{frame}

\begin{frame}{Solution to Practice 3 (Part 2)}
\textbf{Solution (continued):}
\[
\begin{aligned}
  &= \frac{2x^2 + 4x - x^2 + 4}{(x+2)^2} \\
  &= \frac{x^2 + 4x + 4}{(x+2)^2} \\
  &= \frac{(x+2)^2}{(x+2)^2} = 1
\end{aligned}
\]
\end{frame}

\begin{frame}{Solution to Practice 4}
\textbf{Practice 4:}

Find the derivative of $f(x) = \frac{1}{x^2 + 1}$

\textbf{Solution:}
\[
\begin{aligned}
  f'(x) &= -\frac{\frac{d}{dx}(x^2 + 1)}{(x^2 + 1)^2} \\
  &= -\frac{2x}{(x^2 + 1)^2}
\end{aligned}
\]
\end{frame}

\begin{frame}{Solution to Practice 5 (Part 1)}
\textbf{Practice 5:}

Find the derivative of $f(x) = (x^2 + 3x)(x^3 - 2)$

\textbf{Solution:}
\[
\begin{aligned}
  f'(x) &= \frac{d}{dx}(x^2 + 3x) \cdot (x^3 - 2) + (x^2 + 3x) \cdot \frac{d}{dx}(x^3 - 2) \\
  &= (2x + 3) \cdot (x^3 - 2) + (x^2 + 3x) \cdot 3x^2
\end{aligned}
\]
\end{frame}

\begin{frame}{Solution to Practice 5 (Part 2)}
\textbf{Solution (continued):}
\[
\begin{aligned}
  &= 2x^4 - 4x + 3x^3 - 6 + 3x^4 + 9x^3 \\
  &= 5x^4 + 12x^3 - 4x - 6
\end{aligned}
\]
\end{frame}

\begin{frame}{Solution to Practice 6 (Part 1)}
\textbf{Practice 6:}

Find the derivative of $f(x) = \frac{x^3 + 2x}{x^2 - 1}$

\textbf{Solution:}
\[
\begin{aligned}
  f'(x) &= \frac{\frac{d}{dx}(x^3 + 2x) \cdot (x^2 - 1) - (x^3 + 2x) \cdot \frac{d}{dx}(x^2 - 1)}{(x^2 - 1)^2} \\
  &= \frac{(3x^2 + 2) \cdot (x^2 - 1) - (x^3 + 2x) \cdot 2x}{(x^2 - 1)^2}
\end{aligned}
\]
\end{frame}

\begin{frame}{Solution to Practice 6 (Part 2)}
\textbf{Solution (continued):}
\[
\begin{aligned}
  &= \frac{3x^4 - 3x^2 + 2x^2 - 2 - 2x^4 - 4x^2}{(x^2 - 1)^2} \\
  &= \frac{x^4 - 5x^2 - 2}{(x^2 - 1)^2}
\end{aligned}
\]
\end{frame}

\begin{frame}{Solution to Practice 7}
\textbf{Practice 7:}

Find the derivative of $f(x) = (x^2 + 1)^2$

\textbf{Solution:}
\[
\begin{aligned}
  f'(x) &= 2(x^2 + 1) \cdot \frac{d}{dx}(x^2 + 1) \\
  &= 2(x^2 + 1) \cdot 2x \\
  &= 4x(x^2 + 1)
\end{aligned}
\]
\end{frame}

\begin{frame}{Solution to Practice 8}
\textbf{Practice 8:}

Find the derivative of $f(x) = \frac{1}{x^3 + 3x}$

\textbf{Solution:}
\[
\begin{aligned}
  f'(x) &= -\frac{\frac{d}{dx}(x^3 + 3x)}{(x^3 + 3x)^2} \\
  &= -\frac{3x^2 + 3}{(x^3 + 3x)^2} \\
  &= -\frac{3(x^2 + 1)}{(x^3 + 3x)^2}
\end{aligned}
\]
\end{frame}

\begin{frame}{Solution to Practice 9 (Part 1)}
\textbf{Practice 9:}

Find the derivative of $f(x) = x^2 \cdot \sqrt{x^2 + 1}$

\textbf{Solution:}
\[
\begin{aligned}
  f'(x) &= \frac{d}{dx}(x^2) \cdot \sqrt{x^2 + 1} + x^2 \cdot \frac{d}{dx}(\sqrt{x^2 + 1}) \\
  &= 2x \cdot \sqrt{x^2 + 1} + x^2 \cdot \frac{1}{2\sqrt{x^2 + 1}} \cdot 2x
\end{aligned}
\]
\end{frame}

\begin{frame}{Solution to Practice 9 (Part 2)}
\textbf{Solution (continued):}
\[
\begin{aligned}
  &= 2x\sqrt{x^2 + 1} + \frac{x^3}{\sqrt{x^2 + 1}} \\
  &= \frac{2x(x^2 + 1) + x^3}{\sqrt{x^2 + 1}} \\
  &= \frac{2x^3 + 2x + x^3}{\sqrt{x^2 + 1}} \\
  &= \frac{3x^3 + 2x}{\sqrt{x^2 + 1}}
\end{aligned}
\]
\end{frame}

\begin{frame}{Solution to Practice 10 (Part 1)}
\textbf{Practice 10:}

Find the derivative of $f(x) = \frac{\sqrt{x}}{x^2 + 1}$

\textbf{Solution:}
\[
\begin{aligned}
  f'(x) &= \frac{\frac{d}{dx}(\sqrt{x}) \cdot (x^2 + 1) - \sqrt{x} \cdot \frac{d}{dx}(x^2 + 1)}{(x^2 + 1)^2} \\
  &= \frac{\frac{1}{2\sqrt{x}} \cdot (x^2 + 1) - \sqrt{x} \cdot 2x}{(x^2 + 1)^2}
\end{aligned}
\]
\end{frame}

\begin{frame}{Solution to Practice 10 (Part 2)}
\textbf{Solution (continued):}
\[
\begin{aligned}
  &= \frac{\frac{x^2 + 1}{2\sqrt{x}} - 2x\sqrt{x}}{(x^2 + 1)^2} \\
  &= \frac{x^2 + 1 - 4x^2}{2\sqrt{x}(x^2 + 1)^2} \\
  &= \frac{1 - 3x^2}{2\sqrt{x}(x^2 + 1)^2}
\end{aligned}
\]
\end{frame}

\begin{frame}{Solution to Practice 11 (Part 1)}
\textbf{Practice 11:}

Find the derivative of $f(x) = (x^3 - 2x)(x^2 + 3)^2$

\textbf{Solution:}
\[
\begin{aligned}
  f'(x) &= \frac{d}{dx}(x^3 - 2x) \cdot (x^2 + 3)^2 + (x^3 - 2x) \cdot \frac{d}{dx}[(x^2 + 3)^2] \\
  &= (3x^2 - 2) \cdot (x^2 + 3)^2 + (x^3 - 2x) \cdot 2(x^2 + 3) \cdot 2x
\end{aligned}
\]
\end{frame}

\begin{frame}{Solution to Practice 11 (Part 2)}
\textbf{Solution (continued):}
\[
\begin{aligned}
  &= (3x^2 - 2)(x^4 + 6x^2 + 9) + 4x(x^5 - 2x^3 + 3x^3 - 6x) \\
  &= 3x^6 + 18x^4 + 27x^2 - 2x^4 - 12x^2 - 18 + 4x^6 - 8x^4 + 12x^4 - 24x^2 \\
  &= 7x^6 + 26x^4 - 9x^2 - 18
\end{aligned}
\]
\end{frame}

\begin{frame}{Solution to Practice 12}
\textbf{Practice 12:}

Find the derivative of $f(x) = \frac{x^2 - 4}{x^2 + 4}$

\textbf{Solution:}
\[
\begin{aligned}
  f'(x) &= \frac{\frac{d}{dx}(x^2 - 4) \cdot (x^2 + 4) - (x^2 - 4) \cdot \frac{d}{dx}(x^2 + 4)}{(x^2 + 4)^2} \\
  &= \frac{2x \cdot (x^2 + 4) - (x^2 - 4) \cdot 2x}{(x^2 + 4)^2} \\
  &= \frac{2x^3 + 8x - 2x^3 + 8x}{(x^2 + 4)^2} \\
  &= \frac{16x}{(x^2 + 4)^2}
\end{aligned}
\]
\end{frame}

\begin{frame}{Solution to Practice 13}
\textbf{Practice 13:}

Find the derivative of $f(x) = \frac{1}{(x^2 + 1)^2}$

\textbf{Solution:}
\[
\begin{aligned}
  f'(x) &= -\frac{\frac{d}{dx}[(x^2 + 1)^2]}{[(x^2 + 1)^2]^2} \\
  &= -\frac{2(x^2 + 1) \cdot 2x}{(x^2 + 1)^4} \\
  &= -\frac{4x(x^2 + 1)}{(x^2 + 1)^4} \\
  &= -\frac{4x}{(x^2 + 1)^3}
\end{aligned}
\]
\end{frame}

\begin{frame}{Solution to Practice 14 (Part 1)}
\textbf{Practice 14:}

Find the derivative of $f(x) = x \cdot \sqrt{x^2 - 1}$

\textbf{Solution:}
\[
\begin{aligned}
  f'(x) &= \frac{d}{dx}(x) \cdot \sqrt{x^2 - 1} + x \cdot \frac{d}{dx}(\sqrt{x^2 - 1}) \\
  &= 1 \cdot \sqrt{x^2 - 1} + x \cdot \frac{1}{2\sqrt{x^2 - 1}} \cdot 2x
\end{aligned}
\]
\end{frame}

\begin{frame}{Solution to Practice 14 (Part 2)}
\textbf{Solution (continued):}
\[
\begin{aligned}
  &= \sqrt{x^2 - 1} + \frac{x^2}{\sqrt{x^2 - 1}} \\
  &= \frac{x^2 - 1 + x^2}{\sqrt{x^2 - 1}} \\
  &= \frac{2x^2 - 1}{\sqrt{x^2 - 1}}
\end{aligned}
\]
\end{frame}

\begin{frame}{Solution to Practice 15 (Part 1)}
\textbf{Practice 15:}

Find the derivative of $f(x) = \frac{x^3 + x}{x^2 - x + 1}$

\textbf{Solution:}
\[
\begin{aligned}
  f'(x) &= \frac{\frac{d}{dx}(x^3 + x) \cdot (x^2 - x + 1) - (x^3 + x) \cdot \frac{d}{dx}(x^2 - x + 1)}{(x^2 - x + 1)^2} \\
  &= \frac{(3x^2 + 1) \cdot (x^2 - x + 1) - (x^3 + x) \cdot (2x - 1)}{(x^2 - x + 1)^2}
\end{aligned}
\]
\end{frame}

\begin{frame}{Solution to Practice 15 (Part 2)}
\textbf{Solution (continued):}
\[
\begin{aligned}
  &= \frac{3x^4 - 3x^3 + 3x^2 + x^2 - x + 1 - 2x^4 + x^3 - 2x^2 + x}{(x^2 - x + 1)^2} \\
  &= \frac{x^4 - 2x^3 + 2x^2 + 1}{(x^2 - x + 1)^2}
\end{aligned}
\]
\end{frame}

\section{Common Derivatives}

\begin{frame}{Derivatives of Common Functions}
\begin{block}{Power Functions}
\[
\begin{aligned}
  \frac{d}{dx} x^n &= nx^{n-1} \\
  \frac{d}{dx} \sqrt{x} &= \frac{1}{2\sqrt{x}} \\
  \frac{d}{dx} \frac{1}{x} &= -\frac{1}{x^2}
\end{aligned}
\]
\end{block}
\end{frame}

\begin{frame}{Derivatives of Exponential and Logarithmic Functions}
\begin{block}{Exponential and Log}
\[
\begin{aligned}
  \frac{d}{dx} e^x &= e^x \\
  \frac{d}{dx} a^x &= a^x \ln(a) \\
  \frac{d}{dx} \ln(x) &= \frac{1}{x} \\
  \frac{d}{dx} \log_a(x) &= \frac{1}{x \ln(a)}
\end{aligned}
\]
\end{block}
\end{frame}

\begin{frame}{Derivatives of Trigonometric Functions}
\begin{block}{Trigonometric Functions}
\[
\begin{aligned}
  \frac{d}{dx} \sin(x) &= \cos(x) \\
  \frac{d}{dx} \cos(x) &= -\sin(x) \\
  \frac{d}{dx} \tan(x) &= \sec^2(x) \\
  \frac{d}{dx} \cot(x) &= -\csc^2(x) \\
  \frac{d}{dx} \sec(x) &= \sec(x)\tan(x) \\
  \frac{d}{dx} \csc(x) &= -\csc(x)\cot(x)
\end{aligned}
\]
\end{block}
\end{frame}

\begin{frame}{Derivatives of Inverse Trigonometric Functions}
\begin{block}{Inverse Trigonometric Functions}
\[
\begin{aligned}
  \frac{d}{dx} \arcsin(x) &= \frac{1}{\sqrt{1-x^2}} \\
  \frac{d}{dx} \arccos(x) &= -\frac{1}{\sqrt{1-x^2}} \\
  \frac{d}{dx} \arctan(x) &= \frac{1}{1+x^2} \\
  \frac{d}{dx} \arccot(x) &= -\frac{1}{1+x^2} \\
  \frac{d}{dx} \arcsec(x) &= \frac{1}{|x|\sqrt{x^2-1}} \\
  \frac{d}{dx} \arccsc(x) &= -\frac{1}{|x|\sqrt{x^2-1}}
\end{aligned}
\]
\end{block}
\end{frame}

% 新增解答16-25
\begin{frame}{Solution to Practice 16}
\textbf{Practice 16:}

Find the derivative of $f(x) = x^2 \sin(x)$

\textbf{Solution:}
\[
\begin{aligned}
  f'(x) &= \frac{d}{dx}(x^2) \cdot \sin(x) + x^2 \cdot \frac{d}{dx}(\sin(x)) \\
  &= 2x \cdot \sin(x) + x^2 \cdot \cos(x) \\
  &= 2x\sin(x) + x^2\cos(x)
\end{aligned}
\]
\end{frame}

\begin{frame}{Solution to Practice 17}
\textbf{Practice 17:}

Find the derivative of $f(x) = e^x \cos(x)$

\textbf{Solution:}
\[
\begin{aligned}
  f'(x) &= \frac{d}{dx}(e^x) \cdot \cos(x) + e^x \cdot \frac{d}{dx}(\cos(x)) \\
  &= e^x \cdot \cos(x) + e^x \cdot (-\sin(x)) \\
  &= e^x\cos(x) - e^x\sin(x) \\
  &= e^x(\cos(x) - \sin(x))
\end{aligned}
\]
\end{frame}

\begin{frame}{Solution to Practice 18}
\textbf{Practice 18:}

Find the derivative of $f(x) = \ln(x^2 + 1)$

\textbf{Solution:}
\[
\begin{aligned}
  f'(x) &= \frac{1}{x^2 + 1} \cdot \frac{d}{dx}(x^2 + 1) \\
  &= \frac{1}{x^2 + 1} \cdot 2x \\
  &= \frac{2x}{x^2 + 1}
\end{aligned}
\]
\end{frame}

\begin{frame}{Solution to Practice 19}
\textbf{Practice 19:}

Find the derivative of $f(x) = \frac{\sin(x)}{x}$

\textbf{Solution:}
\[
\begin{aligned}
  f'(x) &= \frac{\frac{d}{dx}(\sin(x)) \cdot x - \sin(x) \cdot \frac{d}{dx}(x)}{x^2} \\
  &= \frac{\cos(x) \cdot x - \sin(x) \cdot 1}{x^2} \\
  &= \frac{x\cos(x) - \sin(x)}{x^2}
\end{aligned}
\]
\end{frame}

\begin{frame}{Solution to Practice 20}
\textbf{Practice 20:}

Find the derivative of $f(x) = \arctan(x^2)$

\textbf{Solution:}
\[
\begin{aligned}
  f'(x) &= \frac{1}{1 + (x^2)^2} \cdot \frac{d}{dx}(x^2) \\
  &= \frac{1}{1 + x^4} \cdot 2x \\
  &= \frac{2x}{1 + x^4}
\end{aligned}
\]
\end{frame}

\begin{frame}{Solution to Practice 21}
\textbf{Practice 21:}

Find the derivative of $f(x) = x \cdot e^x$

\textbf{Solution:}
\[
\begin{aligned}
  f'(x) &= \frac{d}{dx}(x) \cdot e^x + x \cdot \frac{d}{dx}(e^x) \\
  &= 1 \cdot e^x + x \cdot e^x \\
  &= e^x + xe^x \\
  &= e^x(1 + x)
\end{aligned}
\]
\end{frame}

\begin{frame}{Solution to Practice 22}
\textbf{Practice 22:}

Find the derivative of $f(x) = \frac{\ln(x)}{x}$

\textbf{Solution:}
\[
\begin{aligned}
  f'(x) &= \frac{\frac{d}{dx}(\ln(x)) \cdot x - \ln(x) \cdot \frac{d}{dx}(x)}{x^2} \\
  &= \frac{\frac{1}{x} \cdot x - \ln(x) \cdot 1}{x^2} \\
  &= \frac{1 - \ln(x)}{x^2}
\end{aligned}
\]
\end{frame}

\begin{frame}{Solution to Practice 23 (Part 1)}
\textbf{Practice 23:}

Find the derivative of $f(x) = \arcsin(\sqrt{x})$

\textbf{Solution:}
\[
\begin{aligned}
  f'(x) &= \frac{1}{\sqrt{1 - (\sqrt{x})^2}} \cdot \frac{d}{dx}(\sqrt{x}) \\
  &= \frac{1}{\sqrt{1 - x}} \cdot \frac{1}{2\sqrt{x}}
\end{aligned}
\]
\end{frame}

\begin{frame}{Solution to Practice 23 (Part 2)}
\textbf{Solution (continued):}
\[
\begin{aligned}
  &= \frac{1}{2\sqrt{x}\sqrt{1 - x}} \\
  &= \frac{1}{2\sqrt{x(1 - x)}}
\end{aligned}
\]
\end{frame}

\begin{frame}{Solution to Practice 24}
\textbf{Practice 24:}

Find the derivative of $f(x) = \sin(x) \cos(x)$

\textbf{Solution:}
\[
\begin{aligned}
  f'(x) &= \frac{d}{dx}(\sin(x)) \cdot \cos(x) + \sin(x) \cdot \frac{d}{dx}(\cos(x)) \\
  &= \cos(x) \cdot \cos(x) + \sin(x) \cdot (-\sin(x)) \\
  &= \cos^2(x) - \sin^2(x) \\
  &= \cos(2x)
\end{aligned}
\]
\end{frame}

\begin{frame}{Solution to Practice 25}
\textbf{Practice 25:}

Find the derivative of $f(x) = \frac{e^x}{x^2 + 1}$

\textbf{Solution:}
\[
\begin{aligned}
  f'(x) &= \frac{\frac{d}{dx}(e^x) \cdot (x^2 + 1) - e^x \cdot \frac{d}{dx}(x^2 + 1)}{(x^2 + 1)^2} \\
  &= \frac{e^x \cdot (x^2 + 1) - e^x \cdot 2x}{(x^2 + 1)^2} \\
  &= \frac{e^x(x^2 + 1 - 2x)}{(x^2 + 1)^2} \\
  &= \frac{e^x(x^2 - 2x + 1)}{(x^2 + 1)^2}
\end{aligned}
\]
\end{frame}

\end{document} 