\documentclass[aspectratio=169]{beamer}
\usepackage{amsmath}
\usepackage{amssymb}
\usepackage{graphicx}
\usepackage{tcolorbox}
\usepackage{booktabs}
\usepackage{colortbl}
\usepackage{xcolor}
\usepackage{tikz}
\usepackage[utf8]{inputenc}

% Custom colors
\definecolor{primary}{RGB}{41, 128, 185}
\definecolor{secondary}{RGB}{52, 152, 219}
\definecolor{accent}{RGB}{231, 76, 60}
\definecolor{lightgray}{RGB}{236, 240, 241}

% Theme customization
\usetheme{Madrid}
\usecolortheme{whale}
\setbeamercolor{structure}{fg=primary}
\setbeamercolor{background canvas}{bg=white}
\setbeamercolor{normal text}{fg=black}

\title{Chapter 5.2: Multiplying and Dividing Rational Expressions}
\subtitle{Rational Expressions - Lesson 2}
\author{Created by Yi-Chen Lin}
\date{\today}

\begin{document}

\begin{frame}
\titlepage
\end{frame}

% I) Multiplying and Dividing Rational Expressions
\begin{frame}{Multiplying and Dividing Rational Expressions}
\begin{tcolorbox}[colback=lightgray,colframe=primary,title=Key Concepts]
\footnotesize
\begin{itemize}
  \item When multiplying rational expressions, add exponents for like variables in the same position (top or bottom).
  \item If a variable appears in both numerator and denominator, subtract/cancel exponents.
  \item When dividing, change division to multiplication and flip (take the reciprocal of) the right-hand fraction only.
  \item After flipping, multiply as usual and simplify.
\end{itemize}
\end{tcolorbox}
\end{frame}

% Multiplying Example
\begin{frame}{Multiplying Example}
\begin{tcolorbox}[colback=lightgray,colframe=secondary,title=Example 1]
\footnotesize
Multiply:
\[
\frac{x^3}{y^2} \times \frac{x^5}{y^3} = \frac{x^{3+5}}{y^{2+3}} = \frac{x^8}{y^5}
\]
\end{tcolorbox}

\begin{tcolorbox}[colback=lightgray,colframe=secondary,title=Example 2]
\footnotesize
Multiply and simplify:
\[
\frac{x^7 y^5}{y^9} \times \frac{x^3}{x^4 y^4} = \frac{x^{7+3} y^5}{x^4 y^{9+4}} = \frac{x^{10} y^5}{x^4 y^{13}} = \frac{x^{6}}{y^{8}}
\]
\end{tcolorbox}
\end{frame}

% Dividing Example
\begin{frame}{Dividing Example}
\begin{tcolorbox}[colback=lightgray,colframe=secondary,title=Example 3]
\footnotesize
Divide:
\[
\frac{a^2 b^3}{c^4} \div \frac{a^4 b}{c^2} = \frac{a^2 b^3}{c^4} \times \frac{c^2}{a^4 b} = \frac{a^{2-4} b^{3-1} c^{2-4}}{1} = \frac{a^{-2} b^{2} c^{-2}}{1} = \frac{b^2}{a^2 c^2}
\]
\end{tcolorbox}
\end{frame}

% Practice: Multiply or Divide
\begin{frame}{Practice: Multiply or Divide}
\begin{tcolorbox}[colback=lightgray,colframe=primary,title=Practice Problems]
\footnotesize
Simplify by multiplying or dividing:
\begin{enumerate}
  \item $\frac{6y^2}{5x} \times \frac{10x^3}{3y}$
  \item $\frac{2x^6}{9} \div \frac{5x^{10}}{6}$
  \item $\frac{15x^2 y^3}{24y^2} \times \frac{6y^5}{5x}$
  \item $\frac{12x^3}{16y^4} \div \frac{7y^2}{14x^2}$
  \item $\frac{45x^3 y^2}{30y^5} \times \frac{18y^4}{75x^2}$
\end{enumerate}
\end{tcolorbox}
\end{frame}

% Practice Solutions
\begin{frame}{Practice Solutions}
\begin{tcolorbox}[colback=lightgray,colframe=accent,title=Detailed Solutions]
\footnotesize
\begin{enumerate}
  \item $\frac{6y^2}{5x} \times \frac{10x^3}{3y} = \frac{6 \times 10 \times y^2 \times x^3}{5 \times 3 \times x \times y} = \frac{60x^3 y^2}{15x y} = \frac{4x^2 y}{1}$
  \item $\frac{2x^6}{9} \div \frac{5x^{10}}{6} = \frac{2x^6}{9} \times \frac{6}{5x^{10}} = \frac{12x^6}{45x^{10}} = \frac{4}{15x^4}$
  \item $\frac{15x^2 y^3}{24y^2} \times \frac{6y^5}{5x} = \frac{15x^2 y^3 \times 6y^5}{24y^2 \times 5x} = \frac{90x^2 y^8}{120x y^2} = \frac{3x y^6}{4}$
  \item $\frac{12x^3}{16y^4} \div \frac{7y^2}{14x^2} = \frac{12x^3}{16y^4} \times \frac{14x^2}{7y^2} = \frac{12x^3 \times 14x^2}{16y^4 \times 7y^2} = \frac{168x^5}{112y^6} = \frac{3x^5}{2y^6}$
  \item $\frac{45x^3 y^2}{30y^5} \times \frac{18y^4}{75x^2} = \frac{45x^3 y^2 \times 18y^4}{30y^5 \times 75x^2} = \frac{810x^3 y^6}{2250x^2 y^5} = \frac{18x y}{50} = \frac{9x y}{25}$
\end{enumerate}
\end{tcolorbox}
\end{frame}

% II) Factoring Rational Expressions
\begin{frame}{Factoring Rational Expressions}
\begin{tcolorbox}[colback=lightgray,colframe=primary,title=Key Concepts]
\footnotesize
\begin{itemize}
  \item When multiplying rational expressions with trinomials, factor every trinomial or difference of squares.
  \item Cancel out any common binomial in both the numerator and denominator.
  \item Always look for NPV's (Non-Permissible Values) from every bracket in the denominator.
\end{itemize}
\end{tcolorbox}
\end{frame}

% Factoring Example
\begin{frame}{Factoring Example}
\begin{tcolorbox}[colback=lightgray,colframe=secondary,title=Example]
\footnotesize
Simplify and state the NPV:
\[
\frac{x^2 + 5x + 6}{x^2 + 3x + 2} \times \frac{x^2 + x - 2}{x^2 + 2x - 3}
\]
Factor:
\[
\frac{(x+2)(x+3)}{(x+1)(x+2)} \times \frac{(x+2)(x-1)}{(x+3)(x-1)}
\]
Cancel common factors:
\[
= \frac{1}{x+1}
\]
NPV: $x \neq -2, -3, -1, 1$
\end{tcolorbox}
\end{frame}

% Practice: Simplify & Find NPV
\begin{frame}{Practice: Simplify & Find NPV}
\begin{tcolorbox}[colback=lightgray,colframe=primary,title=Practice]
\footnotesize
Simplify and find all NPV's:
\begin{enumerate}
  \item $\frac{x^2 - 16}{x^2 - 9} \times \frac{x^2 - 4x + 3}{x^2 - 1}$
  \item $\frac{x^2 - 7x + 12}{x^2 - 4} \div \frac{x^2 - 9}{x^2 - 1}$
\end{enumerate}
\end{tcolorbox}
\end{frame}

% Practice Solutions: NPV
\begin{frame}{Practice Solutions: NPV}
\begin{tcolorbox}[colback=lightgray,colframe=accent,title=Detailed Solutions]
\footnotesize
\begin{enumerate}
  \item $\frac{x^2 - 16}{x^2 - 9} \times \frac{x^2 - 4x + 3}{x^2 - 1}$
  \begin{align*}
    &= \frac{(x-4)(x+4)}{(x-3)(x+3)} \times \frac{(x-3)(x-1)}{(x-1)(x+1)} \\
    &= \frac{(x+4)}{(x+3)(x+1)}
  \end{align*}
  NPV: $x \neq 3, -3, 1, -1$

  \item $\frac{x^2 - 7x + 12}{x^2 - 4} \div \frac{x^2 - 9}{x^2 - 1}$
  \begin{align*}
    &= \frac{(x-3)(x-4)}{(x-2)(x+2)} \times \frac{(x-1)(x+1)}{(x-3)(x+3)} \\
    &= \frac{(x-4)(x-1)(x+1)}{(x-2)(x+2)(x+3)}
  \end{align*}
  NPV: $x \neq 2, -2, 3, -3, 1, -1$
\end{enumerate}
\end{tcolorbox}
\end{frame}

% Extra Practice
\begin{frame}{Extra Practice: Simplify & State NPV}
\begin{tcolorbox}[colback=lightgray,colframe=primary,title=Extra Practice]
\footnotesize
Simplify each of the following and state the NPV's:
\begin{enumerate}
  \item $\frac{x^2 + 3x - 4}{x^2 - 9} \times \frac{x^2 - 4x + 3}{x^2 - 1}$
  \item $\frac{x^2 + 5x + 6}{x^2 - 4} \div \frac{x^2 - 9}{x^2 - 1}$
\end{enumerate}
\end{tcolorbox}
\end{frame}

% Challenge 1
\begin{frame}{Challenge 1: Multiply and Divide}
\begin{tcolorbox}[colback=lightgray,colframe=primary,title=Challenge 1]
\footnotesize
Simplify and state all NPV's:
\[
\frac{x^2-9}{x^2-4} \times \frac{x^2-1}{x^2-5x+6} \div \frac{x^2-4x+3}{x^2-1}
\]
\end{tcolorbox}
\end{frame}

% Challenge 1 Solution - Part 1
\begin{frame}{Challenge 1: Solution (Part 1)}
\begin{tcolorbox}[colback=lightgray,colframe=accent,title=Step-by-Step Solution (Part 1)]
\footnotesize
\textbf{Step 1: Factor all numerators and denominators}
\[
\frac{(x-3)(x+3)}{(x-2)(x+2)} \times \frac{(x-1)(x+1)}{(x-2)(x-3)} \div \frac{(x-1)(x-3)}{(x+1)}
\]

\textbf{Step 2: Change division to multiplication and flip the third fraction}
\[
= \frac{(x-3)(x+3)}{(x-2)(x+2)} \times \frac{(x-1)(x+1)}{(x-2)(x-3)} \times \frac{(x+1)}{(x-1)(x-3)}
\]

\textbf{Step 3: Combine all numerators and denominators}
\[
= \frac{(x-3)(x+3)(x-1)(x+1)(x+1)}{(x-2)(x+2)(x-2)(x-3)(x-1)(x-3)}
\]
\end{tcolorbox}
\end{frame}

% Challenge 1 Solution - Part 2
\begin{frame}{Challenge 1: Solution (Part 2)}
\begin{tcolorbox}[colback=lightgray,colframe=accent,title=Step-by-Step Solution (Part 2)]
\footnotesize
\textbf{Step 4: Cancel common factors}
\[
= \frac{(x+3)(x+1)}{(x-2)(x+2)(x-3)}
\]

\textbf{Step 5: State all NPV's (Non-Permissible Values)}
\begin{itemize}
  \item $x \neq 2, -2, 3, -3, 1, -1$
\end{itemize}
\end{tcolorbox}
\end{frame}

% Challenge 2
\begin{frame}{Challenge 2: Multiply and Divide}
\begin{tcolorbox}[colback=lightgray,colframe=primary,title=Challenge 2]
\footnotesize
Simplify and state all NPV's:
\[
\frac{a^2-4a+3}{a^2-1} \div \frac{a^2-9}{a^2-4} \times \frac{a^2-1}{a^2-2a}
\]
\end{tcolorbox}
\end{frame}

% Challenge 2 Solution - Part 1
\begin{frame}{Challenge 2: Solution (Part 1)}
\begin{tcolorbox}[colback=lightgray,colframe=accent,title=Step-by-Step Solution (Part 1)]
\footnotesize
\textbf{Step 1: Factor all numerators and denominators}
\[
\frac{(a-1)(a-3)}{(a-1)(a+1)} \div \frac{(a-3)(a+3)}{(a-2)(a+2)} \times \frac{(a-1)(a+1)}{a(a-2)}
\]

\textbf{Step 2: Change division to multiplication and flip the second fraction}
\[
= \frac{(a-1)(a-3)}{(a-1)(a+1)} \times \frac{(a-2)(a+2)}{(a-3)(a+3)} \times \frac{(a-1)(a+1)}{a(a-2)}
\]

\textbf{Step 3: Combine all numerators and denominators}
\[
= \frac{(a-1)(a-3)(a-2)(a+2)(a-1)(a+1)}{(a-1)(a+1)(a-3)(a+3)a(a-2)}
\]
\end{tcolorbox}
\end{frame}

% Challenge 2 Solution - Part 2
\begin{frame}{Challenge 2: Solution (Part 2)}
\begin{tcolorbox}[colback=lightgray,colframe=accent,title=Step-by-Step Solution (Part 2)]
\footnotesize
\textbf{Step 4: Cancel common factors}
\[
= \frac{(a+2)(a-1)}{(a+3)a}
\]

\textbf{Step 5: State all NPV's (Non-Permissible Values)}
\begin{itemize}
  \item $a \neq 1, -1, 3, -3, 2, -2, 0$
\end{itemize}
\end{tcolorbox}
\end{frame}

% Challenge 3
\begin{frame}{Challenge 3: Multiply and Divide}
\begin{tcolorbox}[colback=lightgray,colframe=primary,title=Challenge 3]
\footnotesize
Simplify and state all NPV's:
\[
\frac{y^2-16}{y^2-9y+18} \times \frac{y^2-4y+3}{y^2-1} \div \frac{y^2-9}{y^2-4}
\]
\end{tcolorbox}
\end{frame}

% Challenge 3 Solution - Part 1
\begin{frame}{Challenge 3: Solution (Part 1)}
\begin{tcolorbox}[colback=lightgray,colframe=accent,title=Step-by-Step Solution (Part 1)]
\footnotesize
\textbf{Step 1: Factor all numerators and denominators}
\[
\frac{(y-4)(y+4)}{(y-6)(y-3)} \times \frac{(y-1)(y-3)}{(y-1)(y+1)} \div \frac{(y-3)(y+3)}{(y-2)(y+2)}
\]

\textbf{Step 2: Change division to multiplication and flip the third fraction}
\[
= \frac{(y-4)(y+4)}{(y-6)(y-3)} \times \frac{(y-1)(y-3)}{(y-1)(y+1)} \times \frac{(y-2)(y+2)}{(y-3)(y+3)}
\]

\textbf{Step 3: Combine all numerators and denominators}
\[
= \frac{(y-4)(y+4)(y-1)(y-3)(y-2)(y+2)}{(y-6)(y-3)(y-1)(y+1)(y-3)(y+3)}
\]
\end{tcolorbox}
\end{frame}

% Challenge 3 Solution - Part 2
\begin{frame}{Challenge 3: Solution (Part 2)}
\begin{tcolorbox}[colback=lightgray,colframe=accent,title=Step-by-Step Solution (Part 2)]
\footnotesize
\textbf{Step 4: Cancel common factors}
\[
= \frac{(y-4)(y+4)(y-2)}{(y-6)(y+1)(y+3)}
\]

\textbf{Step 5: State all NPV's (Non-Permissible Values)}
\begin{itemize}
  \item $y \neq 6, 3, 1, -1, 4, -4, 2, -2, -3$
\end{itemize}
\end{tcolorbox}
\end{frame}

% Challenge 4
\begin{frame}{Challenge 4: Multiply and Divide}
\begin{tcolorbox}[colback=lightgray,colframe=primary,title=Challenge 4]
\footnotesize
Simplify and state all NPV's:
\[
\frac{m^2-25}{m^2-10m+25} \div \frac{m^2-6m+9}{m^2-1} \times \frac{m^2-1}{m^2-5m}
\]
\end{tcolorbox}
\end{frame}

% Challenge 4 Solution - Part 1
\begin{frame}{Challenge 4: Solution (Part 1)}
\begin{tcolorbox}[colback=lightgray,colframe=accent,title=Step-by-Step Solution (Part 1)]
\footnotesize
\textbf{Step 1: Factor all numerators and denominators}
\[
\frac{(m-5)(m+5)}{(m-5)^2} \div \frac{(m-3)^2}{(m-1)(m+1)} \times \frac{(m-1)(m+1)}{m(m-5)}
\]

\textbf{Step 2: Change division to multiplication and flip the second fraction}
\[
= \frac{(m-5)(m+5)}{(m-5)^2} \times \frac{(m-1)(m+1)}{(m-3)^2} \times \frac{(m-1)(m+1)}{m(m-5)}
\]

\textbf{Step 3: Combine all numerators and denominators}
\[
= \frac{(m-5)(m+5)(m-1)(m+1)(m-1)(m+1)}{(m-5)^2(m-3)^2 m(m-5)}
\]
\end{tcolorbox}
\end{frame}

% Challenge 4 Solution - Part 2
\begin{frame}{Challenge 4: Solution (Part 2)}
\begin{tcolorbox}[colback=lightgray,colframe=accent,title=Step-by-Step Solution (Part 2)]
\footnotesize
\textbf{Step 4: Cancel common factors}
\[
= \frac{(m+5)(m-1)(m+1)}{(m-5)(m-3)^2 m}
\]

\textbf{Step 5: State all NPV's (Non-Permissible Values)}
\begin{itemize}
  \item $m \neq 5, -5, 3, 1, -1, 0$
\end{itemize}
\end{tcolorbox}
\end{frame}

\end{document} 